LeanSubst/Test.lean
@@ -1,0 +1,28 @@
+
+-- namespace Subst
+--   @[simp, coe]
+--   def coe [Coe A B] : Subst A -> Subst B
+--   | σ, n => σ n
+
+--   class CommutesWithSmap (A B) [SubstMap A] [SubstMap B] [c : Coe A B] where
+--     coe_commutes : ∀ a (σ : Subst A), Coe.coe (a[σ]) = (Coe.coe a)[@coe _ _ c σ]
+
+--   @[simp]
+--   theorem coe_cons {a : Subst.Action A} {σ : Subst A} [Coe A B]
+--     : coe (a :: σ) = ↑a :: (coe (B := B) σ)
+--   := by
+--     funext; case _ x =>
+--     simp; cases x <;> simp
+
+--   @[simp]
+--   theorem coe_comp {σ τ : Subst A}
+--     [SubstMap A] [SubstMap B] [Coe A B] [i : CommutesWithSmap A B]
+--     : coe (σ ∘ τ) = coe (B := B) σ ∘ coe τ
+--   := by
+--     funext; case _ x =>
+--     simp [Subst.compose]
+--     generalize zdef : σ x = z at *
+--     cases z <;> simp
+--     case _ a =>
+--       rw [CommutesWithSmap.coe_commutes]
+-- end Subst
